feat: protect `ASCII.Char`, `ASCII.String`, `ASCII.Substring`

ASCII/Char.lean
@@ -7,7 +7,7 @@ import ASCII.Prelude
 namespace ASCII
 
 /-- ASCII character type -/
-structure Char where
+protected structure Char where
   /-- Byte value -/
   toByte : UInt8
   /-- Validity: only 7 bits -/
@@ -18,34 +18,37 @@ instance : Inhabited ASCII.Char := ⟨⟨0, Nat.zero_lt_succ _⟩⟩
 
 namespace Char
 
-@[ext]
-protected theorem ext : {a b : Char} → a.toByte = b.toByte → a = b
-  | ⟨_,_⟩, ⟨_,_⟩, rfl => rfl
+@[ext] protected theorem ext : {a b : ASCII.Char} → a.toByte = b.toByte → a = b
+  | {..}, {..}, rfl => rfl
 
 /-- Underlying ASCII code point as a `Nat` -/
-abbrev toNat (c : Char) := c.toByte.toNat
+abbrev toNat (c : ASCII.Char) := c.toByte.toNat
 
-theorem toNat_lt (c : Char) : c.toNat < 128 := c.valid
+theorem toNat_lt (c : ASCII.Char) : c.toNat < 128 := c.valid
 
 /-- Pack a `Nat` into an ASCII character -/
 @[extern "lean_uint8_of_nat"]
-def ofNatAux (n : @&Nat) (h : n < 128) : Char := ⟨⟨n, Nat.lt_trans h (of_decide_eq_true rfl)⟩, h⟩
+def ofNatAux (n : @&Nat) (h : n < 128) : ASCII.Char :=
+  ⟨⟨n, Nat.lt_trans h (of_decide_eq_true rfl)⟩, h⟩
 
 /-- Convert a `Nat` into an ASCII character
 
   Returns `ASCII.nul` if the `Nat` does not encode a valid ASCII character. -/
 @[noinline, match_pattern]
-def ofNat (n : Nat) : Char := if h : n < 128 then ofNatAux n h else default
+def ofNat (n : Nat) : ASCII.Char := if h : n < 128 then ofNatAux n h else default
 
 /-- Coerce an ASCII character into a Unicode character -/
 @[coe, extern "lean_uint8_to_uint32"]
-protected def toUnicode (c : @&Char) : Unicode.Char where
+protected def toUnicode (c : @&ASCII.Char) : Unicode.Char where
   val := c.toByte.toUInt32
   valid := Or.inl <| c.toByte.toUInt32_toNat ▸ Nat.lt_trans c.toNat_lt (of_decide_eq_true rfl)
 
 instance : Coe ASCII.Char Unicode.Char := ⟨ASCII.Char.toUnicode⟩
 
-theorem toUnicode_isASCII (c : Char) : c.toUnicode.isASCII := by
+instance : ToString ASCII.Char where
+  toString char := char.toUnicode.toString
+
+theorem toUnicode_isASCII (c : ASCII.Char) : c.toUnicode.isASCII := by
   simp [Char.toUnicode, Char.isASCII, _root_.Char.toNat]; exact c.valid
 
 /-- Coerce a Unicode character into an ASCII character -/
@@ -78,70 +81,68 @@ instance : Repr ASCII.Char where
             reprArg char.toNat)))
       prec
 
-instance : ToString ASCII.Char where
-  toString char := char.toUnicode.toString
-
 /-! ## Character Properties -/
 
 /-- Control character -/
-@[inline] def isCntrl (c : Char) :=
+@[inline] def isCntrl (c : ASCII.Char) :=
   c.toByte < 32 || c.toByte == 127
 
 /-- Spacing character -/
-@[inline] def isSpace (c : Char) :=
+@[inline] def isSpace (c : ASCII.Char) :=
   c.toByte == 32 || 9 ≤ c.toByte && c.toByte ≤ 13
 
 /-- Blank character -/
-@[inline] def isBlank (c : Char) :=
+@[inline] def isBlank (c : ASCII.Char) :=
   c.toByte == 32 || c.toByte == 9
 
 /-- Decimal digit -/
-@[inline] def isDigit (c : Char) :=
+@[inline] def isDigit (c : ASCII.Char) :=
   48 ≤ c.toByte && c.toByte ≤ 57
 
 /-- Hexadecimal digit -/
-@[inline] def isXDigit (c : Char) :=
+@[inline] def isXDigit (c : ASCII.Char) :=
   48 ≤ c.toByte && (c.toByte ≤ 57 ||
     65 ≤ c.toByte && (c.toByte ≤ 70 ||
       97 ≤ c.toByte && c.toByte ≤ 102))
 
 /-- Lowercase letter -/
-@[inline] def isLower (c : Char) :=
+@[inline] def isLower (c : ASCII.Char) :=
   97 ≤ c.toByte && c.toByte ≤ 122
 
 /-- Uppercase letter -/
-@[inline] def isUpper (c : Char) :=
+@[inline] def isUpper (c : ASCII.Char) :=
   65 ≤ c.toByte && c.toByte ≤ 90
 
 /-- Alphabetic letter -/
-@[inline] def isAlpha (c : Char) :=
+@[inline] def isAlpha (c : ASCII.Char) :=
   65 ≤ c.toByte && (c.toByte ≤ 90 ||
     97 ≤ c.toByte && c.toByte ≤ 122)
 
 /-- Alphabetic letter or decimal digit -/
-@[inline] def isAlnum (c : Char) :=
+@[inline] def isAlnum (c : ASCII.Char) :=
   48 ≤ c.toByte && (c.toByte ≤ 57 ||
     65 ≤ c.toByte && (c.toByte ≤ 90 ||
       97 ≤ c.toByte && c.toByte ≤ 122))
 
 /-- Punctuation character -/
-@[inline] def isPunct (c : Char) :=
+@[inline] def isPunct (c : ASCII.Char) :=
   33 ≤ c.toByte && (c.toByte ≤ 47 ||
     58 ≤ c.toByte && (c.toByte ≤ 64 ||
       91 ≤ c.toByte && (c.toByte ≤ 96 ||
         123 ≤ c.toByte && c.toByte ≤ 126)))
 
 /-- Graphical character -/
-@[inline] def isGraph (c : Char) :=
+@[inline] def isGraph (c : ASCII.Char) :=
   0x21 ≤ c.toByte && c.toByte ≤ 0x7E
 
 /-- Printable character -/
-@[inline] def isPrint (c : Char) :=
+@[inline] def isPrint (c : ASCII.Char) :=
   0x20 ≤ c.toByte && c.toByte ≤ 0x7E
 
 /-! ## Case Conversion -/
 
-def toLower (c : Char) : Char :=
+/-- Convert uppercase ASCII characters to lowercase -/
+def toLower (c : ASCII.Char) : ASCII.Char :=
   if h : c.isUpper then
     have h : c.toNat + 32 < 128 := by
       simp [isUpper] at h
@@ -152,7 +153,8 @@ def toLower (c : Char) : Char :=
     .ofNatAux _ h
   else c
 
-def toUpper (c : Char) : Char :=
+/-- Convert lowercase ASCII characters to uppercase -/
+def toUpper (c : ASCII.Char) : ASCII.Char :=
   if h : c.isLower then
     have h : c.toNat - 32 < 128 := by
       simp [isLower] at h
@@ -166,105 +168,105 @@ def toUpper (c : Char) : Char :=
 /-! ## Control Characters -/
 
 /-- Null character (ASCII NUL) -/
-protected def nul : Char := ⟨0x00, of_decide_eq_true rfl⟩
+protected def nul : ASCII.Char := ⟨0x00, of_decide_eq_true rfl⟩
 
 /-- Start of Heading (ASCII SOH) -/
-protected def soh : Char := ⟨0x01, of_decide_eq_true rfl⟩
+protected def soh : ASCII.Char := ⟨0x01, of_decide_eq_true rfl⟩
 
 /-- Start of Text (ASCII STX) -/
-protected def stx : Char := ⟨0x02, of_decide_eq_true rfl⟩
+protected def stx : ASCII.Char := ⟨0x02, of_decide_eq_true rfl⟩
 
 /-- End of Text (ASCII ETX) -/
-protected def etx : Char := ⟨0x03, of_decide_eq_true rfl⟩
+protected def etx : ASCII.Char := ⟨0x03, of_decide_eq_true rfl⟩
 
 /-- End of Transmission (ASCII EOT) -/
-protected def eot : Char := ⟨0x04, of_decide_eq_true rfl⟩
+protected def eot : ASCII.Char := ⟨0x04, of_decide_eq_true rfl⟩
 
 /-- Enquiry (ASCII ENQ) -/
-protected def enq : Char := ⟨0x05, of_decide_eq_true rfl⟩
+protected def enq : ASCII.Char := ⟨0x05, of_decide_eq_true rfl⟩
 
 /-- Acknowledge (ASCII ACK) -/
-protected def ack : Char := ⟨0x06, of_decide_eq_true rfl⟩
+protected def ack : ASCII.Char := ⟨0x06, of_decide_eq_true rfl⟩
 
 /-- Bell, Alert (ASCII BEL) -/
-protected def bel : Char := ⟨0x07, of_decide_eq_true rfl⟩
+protected def bel : ASCII.Char := ⟨0x07, of_decide_eq_true rfl⟩
 
 /-- Backspace (ASCII BS) -/
-protected def bs  : Char := ⟨0x08, of_decide_eq_true rfl⟩
+protected def bs  : ASCII.Char := ⟨0x08, of_decide_eq_true rfl⟩
 
 /-- Horizontal Tab (ASCII HT) -/
-protected def ht  : Char := ⟨0x09, of_decide_eq_true rfl⟩
+protected def ht  : ASCII.Char := ⟨0x09, of_decide_eq_true rfl⟩
 
 /-- Line Feed (ASCII LF) -/
-protected def lf  : Char := ⟨0x0A, of_decide_eq_true rfl⟩
+protected def lf  : ASCII.Char := ⟨0x0A, of_decide_eq_true rfl⟩
 
 /-- Vertical Tab (ASCII VT) -/
-protected def vt  : Char := ⟨0x0B, of_decide_eq_true rfl⟩
+protected def vt  : ASCII.Char := ⟨0x0B, of_decide_eq_true rfl⟩
 
 /-- Form Feed (ASCII FF) -/
-protected def ff  : Char := ⟨0x0C, of_decide_eq_true rfl⟩
+protected def ff  : ASCII.Char := ⟨0x0C, of_decide_eq_true rfl⟩
 
 /-- Carriage Return (ASCII CR) -/
-protected def cr  : Char := ⟨0x0D, of_decide_eq_true rfl⟩
+protected def cr  : ASCII.Char := ⟨0x0D, of_decide_eq_true rfl⟩
 
 /-- Shift Out (ASCII SO) -/
-protected def so  : Char := ⟨0x0E, of_decide_eq_true rfl⟩
+protected def so  : ASCII.Char := ⟨0x0E, of_decide_eq_true rfl⟩
 
 /-- Shift In (ASCII SI) -/
-protected def si  : Char := ⟨0x0F, of_decide_eq_true rfl⟩
+protected def si  : ASCII.Char := ⟨0x0F, of_decide_eq_true rfl⟩
 
 /-- Data Link Escape (ASCII DLE) -/
-protected def dle : Char := ⟨0x10, of_decide_eq_true rfl⟩
+protected def dle : ASCII.Char := ⟨0x10, of_decide_eq_true rfl⟩
 
 /-- Device Control One (ASCII DC1, ASCII XON) -/
-protected def dc1 : Char := ⟨0x11, of_decide_eq_true rfl⟩
+protected def dc1 : ASCII.Char := ⟨0x11, of_decide_eq_true rfl⟩
 protected alias xon := Char.dc1
 
 /-- Device Control Two (ASCII DC2) -/
-protected def dc2 : Char := ⟨0x12, of_decide_eq_true rfl⟩
+protected def dc2 : ASCII.Char := ⟨0x12, of_decide_eq_true rfl⟩
 
 /-- Device Control Three (ASCII DC3, ASCII XOFF) -/
-protected def dc3 : Char := ⟨0x13, of_decide_eq_true rfl⟩
+protected def dc3 : ASCII.Char := ⟨0x13, of_decide_eq_true rfl⟩
 protected alias xoff := Char.dc3
 
 /-- Device Control Four (ASCII DC4) -/
-protected def dc4 : Char := ⟨0x14, of_decide_eq_true rfl⟩
+protected def dc4 : ASCII.Char := ⟨0x14, of_decide_eq_true rfl⟩
 
 /-- Negative Acknowledge (ASCII NAK) -/
-protected def nak : Char := ⟨0x15, of_decide_eq_true rfl⟩
+protected def nak : ASCII.Char := ⟨0x15, of_decide_eq_true rfl⟩
 
 /-- Synchronous Idle (ASCII SYN) -/
-protected def syn : Char := ⟨0x16, of_decide_eq_true rfl⟩
+protected def syn : ASCII.Char := ⟨0x16, of_decide_eq_true rfl⟩
 
 /-- End of Transmission Block (ASCII ETB) -/
-protected def etb : Char := ⟨0x17, of_decide_eq_true rfl⟩
+protected def etb : ASCII.Char := ⟨0x17, of_decide_eq_true rfl⟩
 
 /-- Cancel (ASCII CAN) -/
-protected def can : Char := ⟨0x18, of_decide_eq_true rfl⟩
+protected def can : ASCII.Char := ⟨0x18, of_decide_eq_true rfl⟩
 
 /-- End of medium (ASCII EM) -/
-protected def em  : Char := ⟨0x19, of_decide_eq_true rfl⟩
+protected def em  : ASCII.Char := ⟨0x19, of_decide_eq_true rfl⟩
 
 /-- Substitute (ASCII SUB) -/
-protected def sub : Char := ⟨0x1A, of_decide_eq_true rfl⟩
+protected def sub : ASCII.Char := ⟨0x1A, of_decide_eq_true rfl⟩
 
 /-- Escape (ASCII ESC) -/
-protected def esc : Char := ⟨0x1B, of_decide_eq_true rfl⟩
+protected def esc : ASCII.Char := ⟨0x1B, of_decide_eq_true rfl⟩
 
 /-- File Separator (ASCII FS) -/
-protected def fs  : Char := ⟨0x1C, of_decide_eq_true rfl⟩
+protected def fs  : ASCII.Char := ⟨0x1C, of_decide_eq_true rfl⟩
 
 /-- Group Separator (ASCII GS) -/
-protected def gs  : Char := ⟨0x1D, of_decide_eq_true rfl⟩
+protected def gs  : ASCII.Char := ⟨0x1D, of_decide_eq_true rfl⟩
 
 /-- Record Separator (ASCII RS) -/
-protected def rs  : Char := ⟨0x1E, of_decide_eq_true rfl⟩
+protected def rs  : ASCII.Char := ⟨0x1E, of_decide_eq_true rfl⟩
 
 /-- Unit Separator (ASCII US) -/
-protected def us  : Char := ⟨0x1F, of_decide_eq_true rfl⟩
+protected def us  : ASCII.Char := ⟨0x1F, of_decide_eq_true rfl⟩
 
 /-- Space (ASCII SP) -/
-protected def sp  : Char := ⟨0x20, of_decide_eq_true rfl⟩
+protected def sp  : ASCII.Char := ⟨0x20, of_decide_eq_true rfl⟩
 
 /-- Delete (ASCII DEL) -/
-protected def del : Char := ⟨0x7F, of_decide_eq_true rfl⟩
+protected def del : ASCII.Char := ⟨0x7F, of_decide_eq_true rfl⟩
